simplify wf system in Props

def/thm.v
@@ -1,8 +1,7 @@
 From Minirust.def Require Import ty encoding le wf.
 
 Definition mono1 (ty: Ty) :=
-  wf ty
-  -> forall (v1 v2: Value),
+  forall (v1 v2: Value),
   (le v1 v2)
   -> (is_valid_for ty v1)
   -> (is_valid_for ty v2)
@@ -12,22 +11,19 @@ Definition mono1 (ty: Ty) :=
   /\ le v1_l v2_l.
 
 Definition mono2 (ty: Ty) :=
-  wf ty
-  -> forall (l1 l2: list AbstractByte),
+  forall (l1 l2: list AbstractByte),
   (le l1 l2)
   -> le (decode ty l1) (decode ty l2).
 
 Definition rt1 (ty: Ty) :=
-  wf ty
-  -> forall (v: Value),
+  forall (v: Value),
   (is_valid_for ty v)
   -> exists (v_l: list AbstractByte),
   encode ty v = Some v_l
   /\ decode ty v_l = Some v.
 
 Definition rt2 (ty: Ty) :=
-  wf ty
-  -> forall (l: list AbstractByte) (v: Value),
+  forall (l: list AbstractByte) (v: Value),
   (decode ty l = Some v)
   -> exists (v_l: list AbstractByte),
   encode ty v = Some v_l /\ le v_l l.
