proof/bool.v
@@ -1,7 +1,7 @@
 Require Import Coq.Init.Byte List.
 Import ListNotations.
 
-From Minirust.def Require Import ty encoding thm.
+From Minirust.def Require Import ty encoding thm wf.
 From Minirust.proof Require Import defs lemma.le.
 
 Inductive BoolCases1 : list AbstractByte -> Type :=
@@ -43,7 +43,7 @@ Qed.
 Lemma bool_mono1 : mono1 TBool.
 Proof.
 unfold mono1.
-intros _wf v1 v2 HLe valid1 valid2.
+intros v1 v2 HLe valid1 valid2.
 destruct (valid_bool v1 valid1) as [b1 H1].
 destruct (valid_bool v2 valid2) as [b2 H2].
 rewrite H1,H2 in HLe. simpl in HLe.
@@ -57,7 +57,7 @@ Qed.
 Lemma bool_mono2 : mono2 TBool.
 Proof.
 unfold mono2.
-intros _wf l1 l2 HLe.
+intros l1 l2 HLe.
 destruct (mk_le_list _ _ HLe).
 - auto.
 - destruct l.
@@ -78,7 +78,7 @@ Qed.
 Lemma bool_rt1 : rt1 TBool.
 Proof.
 unfold rt1.
-intros _wf v valid.
+intros v valid.
 destruct (valid_bool v valid) as [b H].
 rewrite H. clear H valid v.
 destruct b.
@@ -89,7 +89,7 @@ Qed.
 Lemma bool_rt2 : rt2 TBool.
 Proof.
 unfold rt2.
-intros _wf l v H.
+intros l v H.
 destruct (mk_bool_cases1 l).
 - inversion H. clear v H H1.
   exists [Init x01 None]. simpl. split; reflexivity || auto.
@@ -99,15 +99,15 @@ destruct (mk_bool_cases1 l).
 Qed.
 
 Lemma bool_encode_len : encode_len TBool.
-intros Hwf v l Henc.
+intros v l Henc.
 destruct v; try inversion Henc.
-
 destruct b; inversion Henc; auto.
 Qed.
 
-Lemma bool_props : Props TBool.
+Lemma bool_props (Hwf: wf TBool) : Props TBool.
 Proof.
 split.
+- auto.
 - apply bool_rt1.
 - apply bool_rt2.
 - apply bool_mono1.
