proof/props.v
@@ -1,4 +1,4 @@
-From Minirust.def Require Import ty encoding thm.
+From Minirust.def Require Import ty encoding thm wf.
 From Minirust.proof Require Import defs int bool ptr array.
 Require Import List.
 Import ListNotations.
@@ -6,25 +6,25 @@ Import ListNotations.
 Lemma cheat {P: Prop} : P.
 Admitted.
 
-Lemma gen_props (ty: Ty) : Props ty.
+Lemma gen_props (ty: Ty) : wf ty -> Props ty.
 Proof.
-induction ty.
-- apply bool_props.
-- apply int_props.
-- apply ptr_props.
+induction ty; intros Hwf.
+- apply (bool_props Hwf).
+- apply (int_props Hwf).
+- apply (ptr_props Hwf).
 - apply cheat.
-- apply (array_props IHty).
+- apply (array_props IHty Hwf).
 - apply cheat.
 Qed.
 
-Theorem gen_rt1 (ty: Ty) : rt1 ty.
-Proof. destruct (gen_props ty). assumption. Qed.
+Theorem gen_rt1 (ty: Ty) : wf ty -> rt1 ty.
+Proof. intros Hwf. destruct (gen_props ty); auto. Qed.
 
-Theorem gen_rt2 (ty: Ty) : rt2 ty.
-Proof. destruct (gen_props ty). assumption. Qed.
+Theorem gen_rt2 (ty: Ty) : wf ty -> rt2 ty.
+Proof. intros Hwf. destruct (gen_props ty); auto. Qed.
 
-Theorem gen_mono1 (ty: Ty) : mono1 ty.
-Proof. destruct (gen_props ty). assumption. Qed.
+Theorem gen_mono1 (ty: Ty) : wf ty -> mono1 ty.
+Proof. intros Hwf. destruct (gen_props ty); auto. Qed.
 
-Theorem gen_mono2 (ty: Ty) : mono2 ty.
-Proof. destruct (gen_props ty). assumption. Qed.
+Theorem gen_mono2 (ty: Ty) : wf ty -> mono2 ty.
+Proof. intros Hwf. destruct (gen_props ty); auto. Qed.
